project/inductive/basic/inductive_graph_basic_theory.v
@@ -28,7 +28,7 @@ Require Import MyProject.project.relational_graph_theory.
 
 (* Section to make rewrite work with IG_equiv *)
 (* This proof is based on === being an equivalence relation *)
-Instance IG_Equivalence_eq : Equivalence IG_basic_equiv.
+Instance IG_basic_Equivalence_eq : Equivalence IG_basic_equiv.
 Proof.
   G_derived_equivalence_prover nat unit IG_basic_to_RG_unlE.
 Qed.
@@ -40,7 +40,7 @@ Qed.
 
 
 (* Helper lemma for converting an In (of a map) to an InA, which will eventually be turned to a NatMap.In (which has useful lemmas)  *)
-Lemma In_map_fst_InA : forall (A B: Type) (a : A) (l : list (A * B)),
+Lemma _In_map_fst_InA : forall (A B: Type) (a : A) (l : list (A * B)),
   In a (map fst l) <-> exists (a0 : B), InA (fun (x el : (A * B)) => x = el) (a, a0) l.
 Proof.
   intros. induction l; simpl.
@@ -59,7 +59,7 @@ Qed.
 
 
 (* Conversion from key equality from map to my own (simply written in a slightly different manner) *)
-Lemma In_conditions_same : (NatMap.eq_key_elt (elt:=NatSet.t * NatSet.t)) = (fun x el : Node * (NatSet.t * NatSet.t) => x = el).
+Lemma _In_conditions_same : (NatMap.eq_key_elt (elt:=NatSet.t * NatSet.t)) = (fun x el : Node * (NatSet.t * NatSet.t) => x = el).
 Proof.
   unfold NatMap.eq_key_elt. unfold NatMap.Raw.PX.eqke.
   apply functional_extensionality.
@@ -76,13 +76,13 @@ Qed.
 
 (* This is the most useful one for proving other statements.
   Use it to convert from "use friendly" In- statements to "provable" NatMap.In- statements  *)
-Lemma In_labNodes_is_InMap : forall (x : Node) (ig : IG_basic),
+Lemma _In_labNodes_is_InMap : forall (x : Node) (ig : IG_basic),
   In x (IG_basic_labNodes ig) <-> NatMap.In x ig.
 Proof.
   intros. unfold IG_basic_labNodes.
-  rewrite In_map_fst_InA.
+  rewrite _In_map_fst_InA.
   pose proof (WF.elements_in_iff ig).
-  rewrite In_conditions_same in H.
+  rewrite _In_conditions_same in H.
   specialize H with x.
   symmetry.
   assumption.
@@ -93,12 +93,12 @@ Qed.
 
 
 (* 5 statements on inserting (helpers for mkGraph): update, insEdge, insEdges, insNode, insNodes *)
-Lemma updateEntry_does_not_change_key_set : forall (node : Node) (f : NatSet.t * NatSet.t -> NatSet.t * NatSet.t) (ig : IG_basic) (x : Node),
+Lemma _updateEntry_does_not_change_key_set : forall (node : Node) (f : NatSet.t * NatSet.t -> NatSet.t * NatSet.t) (ig : IG_basic) (x : Node),
   In x (IG_basic_labNodes (_updateEntry node f ig)) <-> In x (IG_basic_labNodes ig).
 Proof.
   intros. unfold _updateEntry.
   destruct (NatMap.find (elt:=NatSet.t * NatSet.t) node ig) eqn:isIn.
-  - rewrite In_labNodes_is_InMap. rewrite In_labNodes_is_InMap. rewrite WF.add_in_iff.
+  - rewrite _In_labNodes_is_InMap. rewrite _In_labNodes_is_InMap. rewrite WF.add_in_iff.
     rewrite WF.in_find_iff. split.
     + intros. destruct H.
       -- rewrite <- H. rewrite isIn. unfold not. intros. discriminate H0.
@@ -108,46 +108,46 @@ Proof.
 Qed.
 
 
-Lemma insEdge_does_not_add_node : forall (edge : (Node * Node)) (ig : IG_basic) (x : Node),
+Lemma _insEdge_does_not_add_node : forall (edge : (Node * Node)) (ig : IG_basic) (x : Node),
   In x (IG_basic_labNodes (_insEdge edge ig)) <-> In x (IG_basic_labNodes ig).
 Proof.
   intros. unfold _insEdge. destruct edge.
   destruct (NatMap.mem (elt:=NatSet.t * NatSet.t) n ig && NatMap.mem (elt:=NatSet.t * NatSet.t) n0 ig) eqn:H0.
-  - rewrite updateEntry_does_not_change_key_set.
-    rewrite updateEntry_does_not_change_key_set.
+  - rewrite _updateEntry_does_not_change_key_set.
+    rewrite _updateEntry_does_not_change_key_set.
     reflexivity.
   - reflexivity.
 Qed.
 
 
-Lemma insEdges_does_not_add_nodes : forall (edges : list (Node * Node)) (ig : IG_basic) (x : Node),
+Lemma _insEdges_does_not_add_nodes : forall (edges : list (Node * Node)) (ig : IG_basic) (x : Node),
   In x (IG_basic_labNodes (_insEdges edges ig)) <-> In x (IG_basic_labNodes ig).
 Proof.
   intros. simpl. induction edges.
   - simpl. reflexivity.
-  - simpl. rewrite insEdge_does_not_add_node. rewrite IHedges. reflexivity.
+  - simpl. rewrite _insEdge_does_not_add_node. rewrite IHedges. reflexivity.
 Qed. 
 
 
-Lemma insNode_any_ins_node : forall (node : Node) (ig : IG_basic) (x : Node),
+Lemma _insNode_any_ins_node : forall (node : Node) (ig : IG_basic) (x : Node),
   In x (IG_basic_labNodes (_insNode node ig)) <-> In x (node :: IG_basic_labNodes ig).
 Proof.
   intros. simpl. unfold _insNode.
-  rewrite In_labNodes_is_InMap. rewrite WF.add_in_iff.
-  rewrite In_labNodes_is_InMap.
+  rewrite _In_labNodes_is_InMap. rewrite WF.add_in_iff.
+  rewrite _In_labNodes_is_InMap.
   reflexivity.
 Qed.  
 
 
-Lemma insNodes_any_ins_all_nodes : forall (nodes : list Node) (ig : IG_basic) (x : Node),
+Lemma _insNodes_any_ins_all_nodes : forall (nodes : list Node) (ig : IG_basic) (x : Node),
   In x (IG_basic_labNodes (_insNodes nodes ig)) <-> In x (nodes ++ IG_basic_labNodes ig).
 Proof.
   intros. induction nodes.
     - simpl. reflexivity.
-    - simpl. rewrite insNode_any_ins_node. simpl. rewrite IHnodes. reflexivity.
+    - simpl. rewrite _insNode_any_ins_node. simpl. rewrite IHnodes. reflexivity.
 Qed.
 
-Lemma insEdge_on_empty_is_empty : forall (edge : Node * Node),
+Lemma _insEdge_on_empty_is_empty : forall (edge : Node * Node),
   _insEdge edge IG_basic_empty = IG_basic_empty.
 (* This proof is very similar to "insEdge_does_not_add_node", but using it here it is more complicated than just doing it again  *)
 Proof.
@@ -158,39 +158,38 @@ Proof.
 Qed. 
 
 
-Lemma insEdges_on_empty_is_empty : forall (edges : list (Node * Node)),
+Lemma _insEdges_on_empty_is_empty : forall (edges : list (Node * Node)),
   _insEdges edges IG_basic_empty = IG_basic_empty.
 (* This proof is very similar to "insEdges_does_not_add_nodes", but using it here it is more complicated than just doing it again  *)
 Proof.
   intros. induction edges; simpl.
   - reflexivity.
-  - rewrite IHedges. rewrite insEdge_on_empty_is_empty. reflexivity.
+  - rewrite IHedges. rewrite _insEdge_on_empty_is_empty. reflexivity.
 Qed.
 
 
 
 (* "big" statement: *)
-Theorem mkGraph_any_ins_all_nodes : forall (nl : list Node) (el : list (Node * Node)) (x : Node),
+Theorem IG_basic_mkGraph_any_ins_all_nodes : forall (nl : list Node) (el : list (Node * Node)) (x : Node),
   In x (IG_basic_labNodes (IG_basic_mkGraph nl el)) <-> In x nl.
 Proof.
-  intros. unfold IG_basic_mkGraph. rewrite insEdges_does_not_add_nodes. rewrite insNodes_any_ins_all_nodes.
+  intros. unfold IG_basic_mkGraph. rewrite _insEdges_does_not_add_nodes. rewrite _insNodes_any_ins_all_nodes.
   rewrite app_nil_r. reflexivity.
 Qed.
 
 
-Theorem empty_isEmpty : IG_basic_isEmpty IG_basic_empty = true.
+Theorem IG_basic_empty_isEmpty : IG_basic_isEmpty IG_basic_empty = true.
 Proof.
   compute. reflexivity.
 Qed.
 
-Theorem labNodes_empty_nil : IG_basic_labNodes IG_basic_empty = [].
+Theorem IG_basic_labNodes_empty_nil : IG_basic_labNodes IG_basic_empty = [].
 Proof.
   compute. reflexivity.
 Qed.
 
 
-(* Protipp: firstorder and congruence seem pretty useful *)
-Lemma not_NatMap_Empty_is_empty_false : forall (A : Type) (m : NatMap.t A), not (NatMap.Empty m) <-> NatMap.is_empty m = false.
+Lemma _not_NatMap_Empty_is_empty_false : forall (A : Type) (m : NatMap.t A), not (NatMap.Empty m) <-> NatMap.is_empty m = false.
 Proof.
   intros. unfold not. rewrite WF.is_empty_iff. destruct (NatMap.is_empty (elt:=A) m) eqn:cond.
   - firstorder. congruence.
@@ -198,22 +197,22 @@ Proof.
 Qed.
 
 
-Theorem  non_empty_isEmpty_false : forall (nodes : list Node) (edges : list (Node * Node)),
+Theorem  IG_basic_non_empty_isEmpty_false : forall (nodes : list Node) (edges : list (Node * Node)),
   length nodes <> 0 <-> IG_basic_isEmpty ((IG_basic_mkGraph nodes edges)) = false.
 Proof.
-  intros. unfold IG_basic_isEmpty. rewrite <- not_NatMap_Empty_is_empty_false. unfold not.
+  intros. unfold IG_basic_isEmpty. rewrite <- _not_NatMap_Empty_is_empty_false. unfold not.
   destruct nodes; simpl; unfold IG_basic_mkGraph.
   - firstorder.
     apply H.
     apply WP.elements_Empty.
 
-    rewrite insEdges_on_empty_is_empty. compute. reflexivity.
+    rewrite _insEdges_on_empty_is_empty. compute. reflexivity.
   - firstorder.
     + apply WP.elements_Empty in H0.
       assert (HH : not (exists e, InA (fun x el : Node * (NatSet.t * NatSet.t) => x = el) (n, e) [])). {
         unfold not. intros. destruct H1. inversion H1.
       }
-      rewrite <- In_conditions_same in HH.
+      rewrite <- _In_conditions_same in HH.
 
       unfold not in HH. apply HH.
       
@@ -222,20 +221,20 @@ Proof.
       rewrite H0 in H2.
       apply H2.
       
-      apply In_labNodes_is_InMap.
-      apply mkGraph_any_ins_all_nodes. simpl. left. reflexivity.
+      apply _In_labNodes_is_InMap.
+      apply IG_basic_mkGraph_any_ins_all_nodes. simpl. left. reflexivity.
     + congruence.
 Qed.
 
 
 
-Theorem matsh_empty_is_nothing : forall (node : Node), IG_basic_match node IG_basic_empty = (None, IG_basic_empty).
+Theorem IG_basic_matsh_empty_is_nothing : forall (node : Node), IG_basic_match node IG_basic_empty = (None, IG_basic_empty).
 Proof.
   intros. compute. reflexivity.
 Qed.
 
 
-Theorem spec4 : forall (node : Node) (nodes : list Node) (edges : list (Node * Node)), 
+Theorem IG_basic_spec4 : forall (node : Node) (nodes : list Node) (edges : list (Node * Node)), 
   In node nodes -> exists froms tos, IG_basic_match node (IG_basic_mkGraph nodes edges) =
   (Some (froms, tos), IG_basic_mkGraph (filter (fun n => negb (node =? n)) nodes) (filter (fun '(from, to) => negb ((from =? node) || (to =? node))) edges)).
 (* This is not even a complete specification and it looks like a hard one to prove... *)
@@ -243,7 +242,7 @@ Proof.
 Admitted.
 
 
-Theorem spec5 : forall (node : Node) (nodes : list Node) (edges : list (Node * Node)), 
+Theorem IG_basic_spec5 : forall (node : Node) (nodes : list Node) (edges : list (Node * Node)), 
   not (In node nodes) -> IG_basic_match node (IG_basic_mkGraph nodes edges) = (None, IG_basic_mkGraph nodes edges).
 Proof.
 Admitted.
