project/relational_graph_IG_operations_theory.v
@@ -18,80 +18,150 @@ Require Import MyProject.project.relational_graph.
 Require Import MyProject.project.relational_graph_IG_operations.
 
 
-
 Open Scope nat_scope.
+
 
 (* Specifies behavior of IH functions on an (edge-label compatible) RG via equational specification *)
 
 
-(* Here start "meaningful statements" *)
-
 (* 5 statements on inserting (helpers for mkGraph): update, insEdge, insEdges, insNode, insNodes *)
 
+
+
 Lemma RG_insEdge_does_not_add_node : forall (A B : Type) (edge : (Edge A B)) (rg : RG A B),
-  RG_labNodes (_insEdge edge rg) = RG_labNodes rg.
+  RG_labNodes (_insEdge edge rg) S== RG_labNodes rg.
 Proof.
-Admitted.
-  (* intros. simpl. unfold RG_labNodes. unfold _insEdge. destruct edge. simpl. reflexivity. *)
+  intros.
+  destruct edge as [[from to] lab]. simpl. unfold RG_labNodes. reflexivity.
+Qed.
 
 
-Lemma RG_insEdges_does_not_add_nodes : forall (A B : Type) (edges : list (@Edge A B)) (rg : RG A B),
-  RG_labNodes (_insEdges edges rg) = RG_labNodes rg.
+
+Lemma RG_insEdges_does_not_add_nodes : forall (A B : Type) (edges : list (Edge A B)) (rg : RG A B),
+  RG_labNodes (_insEdges edges rg) S== RG_labNodes rg.
 Proof.
-Admitted.
+  intros.
+  unfold _insEdges. induction edges; simpl.
+  - reflexivity.
+  - rewrite RG_insEdge_does_not_add_node. rewrite IHedges. reflexivity.
+Qed.
 
+
+
+(* Require Import Coq.Logic.FunctionalExtensionality.
+Require Import Coq.Logic.PropExtensionality.
+
+Ltac breakup_Ensemble_equality :=
+  apply functional_extensionality; intros; apply propositional_extensionality; intros; split. *)
 
 Lemma RG_insNode_any_ins_node : forall (A B : Type) (node : A) (rg : RG A B),
-  RG_labNodes (_insNode node rg) = _customEnsembleAdd node (RG_labNodes rg).
+  RG_labNodes (_insNode node rg) S== cEnsembleAdd node (RG_labNodes rg).
 Proof.
-Admitted.
-
-
+  firstorder.
+Qed.
 
 
 Lemma RG_insNodes_any_ins_all_nodes : forall (A B : Type) (nodes : list A) (rg : RG A B),
-  RG_labNodes (_insNodes nodes rg) = Union A (_listToEnsemble nodes) (RG_labNodes rg).
+  RG_labNodes (_insNodes nodes rg) S== cEnsembleUnion (cListToEnsemble nodes) (RG_labNodes rg).
 Proof.
-Admitted.
+  intros. induction nodes; simpl.
+  - firstorder.
+  - firstorder.
+Qed.
 
 
 
 Lemma RG_insEdge_on_empty_is_empty : forall (A B : Type) (edge : (Edge A B)),
-  _insEdge edge RG_empty = RG_empty.
+  _insEdge edge RG_empty === RG_empty.
 Proof.
-Admitted.
+  intros. unfold RG_equiv. destruct edge as [[from to] lab]. split.
+  - firstorder.
+  - firstorder.
+Qed.
+
 
 
 Lemma RG_insEdges_on_empty_is_empty : forall (A B : Type) (edges : list (Edge A B)),
-  _insEdges edges RG_empty = RG_empty.
-(* This proof is very similar to "insEdges_does_not_add_nodes", but using it here it is more complicated than just doing it again  *)
+  _insEdges edges RG_empty === RG_empty.
 Proof.
-Admitted.
+  intros. pose proof RG_insEdge_on_empty_is_empty. induction edges.
+  - firstorder.
+  - destruct a as [[from to] lab]. firstorder.
+Qed.
+
 
 
 
 (* "big" statement: *)
 Theorem RG_mkGraph_any_ins_all_nodes : forall (A B : Type) (nodes : list A) (edges : list (Edge A B)),
-  RG_labNodes (RG_mkGraph nodes edges) = _listToEnsemble nodes.
+  RG_labNodes (RG_mkGraph nodes edges) S== cListToEnsemble nodes.
 Proof.
-Admitted.
+  intros.
+  unfold RG_mkGraph.
+  rewrite RG_insEdges_does_not_add_nodes.
+  rewrite RG_insNodes_any_ins_all_nodes.
+
+  firstorder.
+Qed.
+
 
 
 Theorem RG_empty_isEmpty : forall (A B : Type), RG_isEmpty (@RG_empty A B).
 Proof.
-  compute. reflexivity.
+  firstorder.
 Qed.
 
-Theorem RG_labNodes_empty_nil : forall (A B : Type), RG_labNodes (@RG_empty A B) = Empty_set A.
+
+
+Theorem RG_labNodes_empty_nil : forall (A B : Type),
+  RG_labNodes (@RG_empty A B) S== Empty_set A.
 Proof.
-Admitted.
+  firstorder.
+Qed.
 
-
-
-Theorem RG_non_empty_isEmpty_false : forall (A B : Type) (nodes : list A) (edges : list (Edge A B)),
-  length nodes <> 0 <-> not (RG_isEmpty ((RG_mkGraph nodes edges))).
+(* Lemma RG_ins_only_edge_isEmpty : forall (A B : Type) (edge : (Edge A B)),
+  _insEdge edge RG_empty === RG_empty.
 Proof.
-Admitted.
+  intros. unfold RG_equiv. destruct edge as [[from to] lab]. split.
+  - firstorder.
+  - firstorder.
+Qed. *)
+
+
+Lemma RG_ins_only_edge_isEmpty : forall (A B : Type) (edge : Edge A B) (rg : RG A B),
+  RG_isEmpty rg <-> RG_isEmpty (_insEdge edge rg).
+Proof.
+  intros. destruct edge as [[from to] lab]. firstorder.
+Qed.
+
+
+Lemma RG_ins_only_edges_isEmpty : forall (A B : Type) (edges : list (Edge A B)) (rg : RG A B),
+  RG_isEmpty rg <-> RG_isEmpty (_insEdges edges rg).
+Proof.
+  intros. induction edges; simpl in *.
+  - reflexivity.
+  - rewrite IHedges. rewrite RG_ins_only_edge_isEmpty. reflexivity.
+Qed.
+
+Lemma RG_insNode_not_isEmpty :  forall (A B : Type) (node : A) (rg : RG A B),
+  not (RG_isEmpty (_insNode node rg)).
+Proof.
+  unfold not. intros. unfold _insNode in H. unfold RG_isEmpty in H. destruct (H node).
+  firstorder.
+Qed.
+
+
+
+
+Theorem RG_insNodes_length_nodes : forall (A B : Type) (nodes : list A) (rg : RG A B),
+  length nodes = 0 <-> RG_isEmpty (_insNodes nodes (@RG_empty _ B)).
+Proof.
+  intros. destruct nodes.
+  - firstorder.
+  - simpl. split; intros.
+    + discriminate H.
+    + pose proof RG_insNode_not_isEmpty. unfold not in H0. apply H0 in H. destruct H.
+Qed.
 
 
 
@@ -100,7 +170,6 @@ Theorem RG_match_empty_is_nothing : forall (A B : Type) (node : A),
   RG_match node (@RG_empty A B) = ((False, (fun x y => False, node, fun x y => False)), RG_empty).
 Proof.
 Admitted.
-
 
 
 
